Provisional proof of addMoneyToAccountPositive

isabelle/PositiveAccounts.thy
@@ -2,29 +2,62 @@ theory PositiveAccounts
 imports Semantics
 begin
 
-theorem accountsArePositive :
-  "(\<forall>x. moneyInAccount x (accounts state) \<ge> 0) \<Longrightarrow>
-   computeTransaction txIn state cont = TransactionOutput txOut \<Longrightarrow>
-   moneyInAccount y (accounts (txOutState txOut)) \<ge> 0"
-  oops
+lemma addMoneyToAccountPositve_match :
+ "\<forall>x. 0 \<le> moneyInAccount x accs \<Longrightarrow>
+    money > 0 \<Longrightarrow>
+    newBalance > 0 \<Longrightarrow>
+    0 \<le> moneyInAccount y (MList.insert y newBalance accs)"
+  apply simp
+  by (simp add: MList.insert_lookup_Some)
+
+lemma addMoneyToAccountPositive_noMatch :
+ "\<forall>x. 0 \<le> moneyInAccount x accs \<Longrightarrow>
+    money > 0 \<Longrightarrow>
+    accId \<noteq> y \<Longrightarrow>
+    newBalance > 0 \<Longrightarrow>
+    0 \<le> moneyInAccount y (MList.insert accId newBalance accs)"
+  apply simp
+  by (simp add: insert_lookup_different)
+
+lemma addMoneyToAccountPositive :
+  "0 \<le> money \<Longrightarrow> (\<forall>x. moneyInAccount x accs \<ge> 0)
+  \<Longrightarrow> moneyInAccount y (addMoneyToAccount accId money accs) \<ge> 0"
+  apply (simp only:"addMoneyToAccount.simps")
+  apply (cases "money \<le> 0")
+  apply simp
+  apply (simp del:moneyInAccount.simps)
+  apply (cases "accId = y")
+  apply (metis (full_types) addMoneyToAccountPositve_match add_le_same_cancel1 dual_order.trans not_less)
+proof -
+  assume a1: "accId \<noteq> y"
+assume a2: "\<not> money \<le> 0"
+  assume a3: "\<forall>x. 0 \<le> moneyInAccount x accs"
+  then have f4: "\<not> moneyInAccount accId accs + money \<le> 0"
+using a2 by (meson add_le_same_cancel1 le_less_trans not_less)
+  have "\<And>i. \<not> 0 < i \<or> 0 \<le> moneyInAccount y (MList.insert accId i accs)"
+    using a3 a1 addMoneyToAccountPositive_noMatch by blast
+then show "0 \<le> moneyInAccount y (let i = moneyInAccount accId accs + money in if i \<le> 0 then MList.delete accId accs else MList.insert accId i accs)"
+  using f4 by auto
+qed
+
 
 (* Alternative formulation *)
 
 fun allAccountsPositive :: "(AccountId \<times> Money) list \<Rightarrow> bool" where
-"allAccountsPositive accs = foldl (\<lambda> r (_, money) . r \<and> money \<ge> 0) True accs"
-
+"allAccountsPositive accs = foldl (\<lambda> r (_, money) . r \<and> money > 0) True accs"
 
 fun allAccountsPositiveState :: "State \<Rightarrow> bool" where
 "allAccountsPositiveState state = allAccountsPositive (accounts state)"
 
 lemma positiveMoneyInAccount :
-  "allAccountsPositive accs \<Longrightarrow> 0 \<le> moneyInAccount accId accs"
+  "allAccountsPositive accs \<Longrightarrow> 0 < moneyInAccount accId accs"
   oops
 
 lemma addMoneyToAccountPositive :
   "0 \<le> money \<and> allAccountsPositive accs
   \<Longrightarrow> allAccountsPositive (addMoneyToAccount accId money accs)"
   oops
+
 
 theorem accountsArePositive2 :
     "allAccountsPositiveState state
